

HW ~ 1.

$$\textcircled{4.} \quad A = \begin{pmatrix} 1 & 10 \\ \delta & 1 \end{pmatrix}$$

$\Downarrow$

$$1. (1-\lambda)^2 - 10\delta = 0$$

$$1-\lambda = \pm \sqrt{10\delta}$$

$$\lambda_1 = 1 + \sqrt{10\delta}$$

$$\lambda_2 = 1 - \sqrt{10\delta}$$

$$\Rightarrow E(\delta) = 1 + \sqrt{10\delta}$$

$$2. dE(\delta) = \sqrt{10} \frac{d\delta}{2\sqrt{\delta}}$$

$\Downarrow$

$$K(\delta) = \frac{dE(\delta)}{d\delta} = \frac{\sqrt{10}}{2\sqrt{\delta}}$$

$\Downarrow$

$$3. K(10) = \frac{1}{2} ; K(0,1) = 5 //$$

$$\textcircled{1.} \quad 1. \mathcal{L}_n(\alpha) = \int_0^1 \frac{x^n}{x+\alpha} dx = \int_0^1 \frac{x^n + \alpha x^{n-1} - \alpha x^{n-1}}{x+\alpha} dx =$$

$$= \int_0^1 x^{n-1} dx - \int_0^1 \frac{\alpha x^{n-1}}{x+\alpha} dx = \frac{1}{n} - \alpha \mathcal{L}_{n-1}$$

$\Downarrow$

$$\mathcal{L}_n = \frac{1}{n} - \alpha \mathcal{L}_{n-1} //$$

$$2. \mathcal{L}_0(\alpha) = \int_0^1 \frac{1}{x+\alpha} dx = \ln \left| \frac{x+\alpha}{\alpha} \right| //$$

3. —